\documentclass{ximera}

\input{../preamble.tex}


\title[Dig-In:]{The Product rule and quotient rule}

\begin{document}
\begin{abstract}
Here we compute derivatives of products and quotients of functions
\end{abstract}
\maketitle


\section{The product rule}


Consider the product of two simple functions, say
\[
f(x)\cdot g(x)
\]
where $f(x)=x^2+1$ and $g(x)=x^3-3x$. An obvious guess for the
derivative of $f(x)g(x)$ is the product of the derivatives:
\begin{align*}
f'(x)g'(x) &= (2x)(3x^2-3)\\
&= 6x^3-6x.
\end{align*}
Is this guess correct? We can check by rewriting $f$ and $g$ and doing
the calculation in a way that is known to work. Write with me
\begin{align*}
f(x)g(x) &= (x^2+1)(x^3-3x)\\
&=x^5-3x^3+x^3-3x\\
&=x^5-2x^3-3x.
\end{align*} 
Hence
\[
\ddx f(x) g(x) = \ddx(x^5 - 2x^3 - 3x) = 5x^4-6x^2-3, 
\]
so we see that 
\[
\ddx f(x) g(x) \ne  f'(x)g'(x).
\]
So the derivative of $f(x)g(x)$ is \textbf{not} as simple as
$f'(x)g'(x)$. Never fear, we have a rule for exactly this
situation.
\begin{theorem}[The product rule]\index{derivative rules!product}\index{product rule}\label{theorem:product-rule}
If $f$ and $g$ are differentiable, then
\[
\ddx f(x)g(x) = f(x)g'(x)+f'(x)g(x).
\]
\end{theorem}

%% \begin{image}
%% \begin{tikzpicture}
%% 	\begin{axis}[
%%             clip=false,
%%             domain=1.5:6, 
%%             ytickmin=1,ytickmax=0,
%%             xtick={4},ytickmin=1,ytickmax=0,
%%             xticklabels={$a$},
%%             ymin=0, ymax=6,
%%             xlabel=$x$, ylabel=$y$,
%%             axis lines=center,
%%             every axis y label/.style={at=(current axis.above origin),anchor=south},
%%             every axis x label/.style={at=(current axis.right of origin),anchor=west},
%%             axis on top,
%%           ]          
%%           %\addplot [dashed, textColor] plot coordinates {(4,0) (4,3.08)};
%%           %\node at (axis cs:4,0) [anchor=north] {$x$};

%%           \addplot [penColor5,very thick] plot coordinates {(5,1.4) (5,1.9)};
%%           \addplot [dashed, very thick, textColor] plot coordinates {(4,1.4) (5,1.4)};

%%           \addplot [penColor4,very thick] plot coordinates {(5,2.2) (5,2.6)};
%%           \addplot [dashed, very thick, textColor] plot coordinates {(4,2.2) (5,2.2)};

%%           \addplot [very thick, penColor5!50!penColor2] plot coordinates {(5,3.08) (5,4.18)};
%%           \addplot [very thick, penColor4!50!penColor] plot coordinates {(5,4.18) (5,4.74)};
%%           \addplot [dashed, very thick, textColor] plot coordinates {(4,3.08) (5,3.08)};
        
%%           \addplot [very thick,penColor,smooth] {-.6+.5*x};
%%           \addplot [very thick,penColor2,smooth] {.6+.4*x};         
%%           \addplot [very thick,penColor3,smooth,domain=1:5.5] {-.36+.06*x+.2*x^2};      
%%           \addplot [penColor3!70!background,smooth, domain=1.6:5.6] {-3.56+1.66*x};      
          
%%           \addplot [dashed, textColor] plot coordinates {(4,0) (4,3.08)};

%%           \node at (axis cs:3.5,1.1) [anchor=north,penColor] {$f(x)$};
%%           \node at (axis cs:2,1.95) [anchor=north,penColor2] {$g(x)$};
%%           \node at (axis cs:4.7,4.3) [anchor=east,penColor3] {$f(x)g(x)$};

%%           \node at (axis cs:5,3.91) [anchor=west] {${\color{penColor}f(a)}{\color{penColor4}g'(a)h}+{\color{penColor5}f'(a)h}{\color{penColor2}g(a)} + {\color{penColor5}f'(a)h}{\color{penColor4}g'(a)h}$};
%%           \node at (axis cs:5,1.65) [anchor=west,penColor5] {$f'(a)h$};
%%           \node at (axis cs:5,2.4) [anchor=west,penColor4] {$g'(a)h$};
%%           \node at (axis cs:4.5,1.5) [anchor=north] {$\underbrace{\hspace{.40in}}_{h}$};

%%           \addplot[color=penColor,fill=penColor,only marks,mark=*] coordinates{(4,1.4)};  %% closed hole          
%%           \addplot[color=penColor2,fill=penColor2,only marks,mark=*] coordinates{(4,2.2)};  %% closed hole          
%%           \addplot[color=penColor3,fill=penColor3,only marks,mark=*] coordinates{(4,3.08)};  %% closed hole          
%%         \end{axis}
%% \end{tikzpicture}
%% %% \caption[A geometric interpretation of the product rule.]{A geometric interpretation of the product rule. Since every
%% %%   point on $f(x)g(x)$ is the product of the corresponding points on
%% %%   $f(x)$ and $g(x)$, increasing $a$ by a ``small amount'' $h$,
%% %%   increases $f(a)g(a)$ by the sum of $f(a)g'(a)h$ and
%% %%   $f'(a)hg(a)$. Hence,
%% %% \begin{align*}
%% %% \frac{\Delta y}{\Delta x} &\approx \frac{f(a)g'(a)h+f'(a)g(a)h + f'(a)g'(a)h^2}{h}\\
%% %% &\approx f(a)g'(a) + f'(a)g(a).
%% %% \end{align*}}
%% \end{image}

%% \begin{explanation}
%% From the limit definition of the derivative, write
%% \[
%% \ddx (f(x)g(x)) = \lim_{h \to0} \frac{f(\answer[given]{x+h})g(\answer[given]{x+h}) - f(\answer[given]{x})g(\answer[given]{x})}{\answer[given]{h}}
%% \]
%% Now we use a trick, we add $0 = -f(x+h)g(x) + f(x+h)g(x)$:
%% \begin{align*}
%% &=\lim_{h \to0} \frac{f(x+h)g(x+h){\color{penColor2}-f(x+h)g(x) + f(x+h)g(x)}- f(x)g(x)}{h} \\ 
%% &=\lim_{h \to0} \frac{f(x+h)g(x+h)-f(x+h)g(x)}{h} + \lim_{h \to0} \frac{f(x+h)g(x)- f(x)g(x)}{h}.
%% \end{align*}
%% Since both $f(x)$ and $g(x)$ are differentiable, they are
%% continuous, see Theorem~\ref{theorem:diff-cont}. Hence
%% \begin{align*}
%% &=\lim_{h \to0} \left(f(x+h)\frac{g(x+h)-g(x)}{h}\right) + \lim_{h \to0} \left(\frac{f(x+h)- f(x)}{h}g(x)\right) \\ 
%% &=\lim_{h \to0} f(x+h)\lim_{h \to0}\cdot \frac{g(x+h)-g(x)}{h} + \lim_{h \to0} \frac{f(x+h)- f(x)}{h} \cdot \lim_{h \to0}g(x) \\ 
%% &=f(x)g'(x) + f'(x)g(x).
%% \end{align*}
%% \end{explanation}



Let's return to the example with which we started.
\begin{example} 
Let $f(x)=(x^2+1)$ and $g(x)=(x^3-3x)$. Compute:
\[
\ddx f(x)g(x)
\]

\begin{explanation}
Write with me
\begin{align*}
\ddx f(x)g(x) &= f(x)g'(x) + f'(x)g(x)\\
&=(x^2+1)(\answer[given]{3x^2-3}) + (\answer[given]{2x})(x^3-3x).
\end{align*}
We could stop here, but we should show that expanding this out recovers
our previous result. Write with me
\begin{align*}
(x^2+1)&(3x^2-3) + 2x(x^3-3x)\\
  &= 3x^4-3x^2 +3x^2 -3 + 2x^4-6x^2\\
&=\answer[given]{5x^4-6x^2-3},
\end{align*}
which is precisely what we obtained before.
\end{explanation}
\end{example}

Now that we are pros, let's try one more example.



\section{The quotient rule}


We'd like to have a formula to compute
\[
\ddx \frac{f(x)}{g(x)}
\]
if we already know $f'(x)$ and $g'(x)$. Instead of attacking this
problem head-on, let's notice that we've already done part of the
problem: $f(x)/g(x)= f(x)\cdot(1/g(x))$, that is, this is really a
product, and we can compute the derivative if we know $f'(x)$ and
$(1/g(x))'$. This brings us to our next derivative rule.

\begin{theorem}[The quotient rule]\index{derivative rules!quotient}\index{quotient rule}\label{theorem:quotient-rule}
If $f$ and $g$ are differentiable, then
\[
\ddx \frac{f(x)}{g(x)} = \frac{f'(x)g(x)-f(x)g'(x)}{g(x)^2}.
\]
\end{theorem}
%% \begin{explanation}
%% First note that if we knew how to compute
%% \[
%% \ddx \frac{1}{g(x)}
%% \]
%% then we could use the product rule to complete our explanation.  Write
%% \begin{align*}
%% \ddx\frac{1}{g(x)}&=\lim_{h\to0} \frac{\frac{1}{g(x+h)}-\frac{1}{g(x)}}{h} \\
%% &=\lim_{h\to0} \frac{\frac{g(\answer[given]{x})-g(\answer[given]{x+h})}{g(x+h)g(x)}}{h} \\
%% &=\lim_{h\to0} \frac{g(x)-g(x+h)}{g(x+h)g(x)h} \\
%% &=\lim_{h\to0} -\frac{g(x+h)-g(x)}{h} \frac{1}{g(x+h)g(x)} \\
%% &=-\frac{g'(x)}{g(x)^2}.
%% \end{align*}
%% Now we can put this together with the product rule:
%% \begin{align*}
%% \ddx\frac{f(x)}{g(x)} &=f(x)\frac{-g'(x)}{g(x)^2}+f'(x)\frac{1}{g(x)}\\
%% &=\frac{-f(x)g'(x)+f'(x)g(x)}{g(x)^2}\\
%% &=\frac{f'(x)g(x)-f(x)g'(x)}{g(x)^2}.
%% \end{align*}

%% \end{explanation}


\begin{example}
Compute:
\[
\ddx \frac{x^2+1}{x^3-3x}
\]

\begin{explanation}
Write with me
\begin{align*}
\ddx \frac{x^2+1}{x^3-3x} &= \frac{2x(\answer[given]{x^3-3x})-(\answer[given]{x^2+1})(3x^2-3)}{(\answer[given]{x^3-3x})^2}\\
&=\frac{-x^4-6x^2+3}{(\answer[given]{x^3-3x})^2}.
\end{align*}
\end{explanation}
\end{example}

It is often possible to calculate derivatives in more than one way, as
we have already seen. Since every quotient can be written as a
product, it is always possible to use the product rule to compute the
derivative, though it is not always simpler.

\begin{example}
Compute: 
\[
\ddx \frac{625-x^2}{\sqrt{x}}
\] 
in two ways. First using the quotient rule and then using the product
rule.
\begin{explanation}
First, we'll compute the derivative using the quotient rule. Write with me
\[
\ddx \frac{625-x^2}{\sqrt{x}} = \frac{\left(-2x\right)\left(\answer[given]{\sqrt{x}}\right) - (\answer[given]{625-x^2})\left(\frac{1}{2}x^{-1/2}\right)}{\answer[given]{x}}.
\]

Second, we'll compute the derivative using the product rule:
\begin{align*}
\ddx \frac{625-x^2}{\sqrt{x}} &= \ddx \left(625-x^2\right)x^{-1/2}\\
=\left(625-x^2\right)&\left(\answer[given]{\frac{-x^{-3/2}}{2}}\right)+ (\answer[given]{-2x})\left(x^{-1/2}\right).
\end{align*}
With a bit of algebra, both of these simplify to
\[
-\frac{3x^2+625}{2x^{3/2}}.
\]
\end{explanation}
\end{example}


\end{document}
